code/ecdsap256sha2/Hacl.Impl.ECDSA.fsti
@@ -32,7 +32,7 @@ open Hacl.Impl.ECDSA.P256SHA256.KeyGeneration
 open Hacl.Impl.ECDSA.P256SHA256.Signature
 open Hacl.Impl.ECDSA.P256SHA256.Verification
 
-
+(*
 val ecdsa_p256_sha2_keyGen: 
     result: lbuffer uint8 (size 64) 
   -> privKey: lbuffer uint8 (size 32) 
@@ -54,82 +54,34 @@ val ecdsa_p256_sha2_keyGen:
         publicKeyY == yN
       )
     )
+*)
 
-
-val ecdsa_p256_sha2_sign: 
-    result: lbuffer uint8 (size 64) 
-  -> mLen: size_t 
-  -> m: lbuffer uint8 mLen 
-  -> privKey: lbuffer uint8 (size 32) 
-  -> k: lbuffer uint8 (size 32) 
-  -> Stack uint64
-  (requires fun h ->
+val ecdsa_p256_sha2_sign: result: lbuffer uint8 (size 64) -> mLen: size_t -> m: lbuffer uint8 mLen ->
+  privKey: lbuffer uint8 (size 32) -> 
+  k: lbuffer uint8 (size 32) -> 
+  Stack uint64
+  (requires fun h -> 
     live h result /\ live h m /\ live h privKey /\ live h k /\
     disjoint result m /\
     disjoint result privKey /\
     disjoint result k /\
-    nat_from_bytes_le (as_seq h privKey) < prime_p256_order /\
-    nat_from_bytes_le (as_seq h k) < prime_p256_order
+    nat_from_bytes_be (as_seq h privKey) < prime_p256_order /\
+    nat_from_bytes_be (as_seq h k) < prime_p256_order
   )
-  (ensures fun h0 flag h1 ->
-    assert_norm (pow2 32 < pow2 61);
+  (ensures fun h0 flag h1 -> 
     modifies (loc result) h0 h1 /\
-     (
-      let resultR = gsub result (size 0) (size 32) in
-      let resultS = gsub result (size 32) (size 32) in
-      let r, s, flagSpec = Hacl.Spec.ECDSA.ecdsa_signature (uint_v mLen) (as_seq h0 m) (as_seq h0 privKey) (as_seq h0 k) in
-      let resultR = nat_from_bytes_le (as_seq h1 resultR) in
-      let resultS = nat_from_bytes_le (as_seq h1 resultS) in
-      flag == flagSpec /\ r == resultR /\ s == resultS
-    )
-  )
-
-
-val ecdsa_p256_sha2_sign_nist: 
-    result: lbuffer uint8 (size 64) 
-  -> m: lbuffer uint8 (size 32) 
-  -> privKey: lbuffer uint8 (size 32) 
-  -> k: lbuffer uint8 (size 32) 
-  -> Stack uint64
-  (requires fun h ->
-    live h result /\ live h m /\ live h privKey /\ live h k /\
-    LowStar.Monotonic.Buffer.all_disjoint [loc result; loc m; loc privKey; loc k] /\
-    nat_from_bytes_le (as_seq h m) < prime_p256_order /\
-    nat_from_bytes_le (as_seq h privKey) < prime_p256_order /\
-    nat_from_bytes_le (as_seq h k) < prime_p256_order
-  )
-  (ensures fun h0 flag h1 ->
-    modifies (loc result) h0 h1 /\
-    (
-      let resultR = gsub result (size 0) (size 32) in
-      let resultS = gsub result (size 32) (size 32) in
-      let r, s, flagSpec = Hacl.Spec.ECDSA.ecdsa_signature_nist_compliant (as_seq h0 m) (as_seq h0 privKey) (as_seq h0 k) in
-      let resultR = nat_from_bytes_le (as_seq h1 resultR) in
-      let resultS = nat_from_bytes_le (as_seq h1 resultS) in
-      flag == flagSpec /\ r == resultR /\ s == resultS
-    )
+     (assert_norm (pow2 32 < pow2 61);
+      let resultR = gsub result (size 0) (size 32) in 
+      let resultS = gsub result (size 32) (size 32) in 
+      let r, s, flagSpec = Hacl.Spec.ECDSA.ecdsa_signature (uint_v mLen) (as_seq h0 m) (as_seq h0 privKey) (as_seq h0 k) in 
+      as_seq h1 resultR == nat_to_bytes_be 32 r /\
+      as_seq h1 resultS == nat_to_bytes_be 32 s /\
+      flag == flagSpec 
+    )    
   )
 
 (* This code is not side channel resistant *)
 val ecdsa_p256_sha2_verify:
-    mLen:size_t
-  -> m:lbuffer uint8 mLen
-  -> pubKey: lbuffer uint64 (size 8)
-  -> r: lbuffer uint64 (size 4)
-  -> s: lbuffer uint64 (size 4) ->
-  Stack bool
-    (requires fun h -> live h pubKey /\ live h r /\ live h s /\ live h m)
-    (ensures fun h0 result h1 ->
-      modifies0 h0 h1 /\
-      (
-        let pubKeyX = as_nat h0 (gsub pubKey (size 0) (size 4)) in
-        let pubKeyY = as_nat h0 (gsub pubKey (size 4) (size 4)) in
-        result == Hacl.Spec.ECDSA.ecdsa_verification (pubKeyX, pubKeyY) (as_nat h0 r) (as_nat h0 s) (v mLen) (as_seq h0 m)
-      )
-    )
-
-(* This code is not side channel resistant *)
-val ecdsa_p256_sha2_verify_u8:
     mLen: size_t
   -> m: lbuffer uint8 mLen
   -> pubKey: lbuffer uint8 (size 64)
